hello

handout2.dfy
@@ -1,6 +1,26 @@
 class Row {
-Var name.String
-Var age.int
+	var name:array<char>;
+ 	var age:int; 
+
+	constructor ()
+ 	{ name := new char[0] ; age := 0; }
+
+
+ 	method setName(a:array<char>)
+ 	modifies this
+ 	requires a.Length > 0
+ 	ensures this.name.Length > 0
+ 	{
+ 		this.name := a;
+ 	}
+
+ 	method setAge(n:int)
+ 	modifies this
+ 	requires n >= 0;
+ 	ensures this.age >= 0;
+ 	{
+		this.age := n; 		
+ 	}
 }
 
 class PersonDB
@@ -14,22 +34,42 @@ class PersonDB
         size := 0;
     }
 
-    method add() 
-     modifies people, this.size
+    method add() returns(pos:int)
+    modifies this.people
+    requires this.size < this.people.Length
     {
         if( 0 <= size < people.Length ) 
         {
             people[size] := new Row();
             size := size + 1;
         }
+        pos := size-1;
     }
 
     method delete(i:int) 
-     modifies people, this.size
+    modifies this.people
     {
-        if( 0 <= i < a.Length )
+        if( 0 <= i < people.Length )
+        {
             people[i] := null;
+        }
     }
+
+    method find(i:int) returns (p:Person)
+    requires 0 < i < size    
+ 	{
+ 		p := null;
+ 		if( people[i] != null)
+        {
+	 		if(people[i].name.Length > 0 && people[i].age >= 0)
+	 		{
+		 		p := new Person();
+		 		p.setAge(people[i].age);
+		 		p.setName(people[i].name);
+		 		p.setDB(this);
+	 		}
+        }
+ 	}
 }
 
 
@@ -38,50 +78,88 @@ class Person
 	var id:int;
  	var name:array<char>; 
 	var age:int;
-	var c:PersonDB;
+	var con:PersonDB;
 
- 	function Transiet():bool
+ 	function Transient():bool
  	reads this
- 	{ name != "" c == null id == -1}
+ 	{ con == null && id == -1 }
  	
  	function Persitent():bool
  	reads this
- 	{ id > -1 && c != null } 
+ 	{ id > -1 && con != null } 
 
  	function Detatched():bool
  	reads this
- 	{ } 
+ 	{ id > -1 && con == null} 
 
 	constructor ()
- 	ensures Transiet()
- 	{ id := -1; name := ""; age := 0; c := null; }
+ 	ensures Transient()
+ 	{ id := -1; name := new char[0]; age := 0; con := null; }
 
- 	method find(PersondDB c)
- 	ensures Persitent()
- 	{ }
-
- 	method save(PersondDB c)
+ 	method save(c:PersonDB)
  	modifies this
+ 	requires this.name.Length > 0
+ 	requires this.age >= 0
+ 	requires c.size < c.people.Length
+ 	requires Transient() || Persitent()
  	ensures Persitent()
  	{	
- 		c.add()
+ 		var pos := c.add();
+ 		c.people[pos].setName(this.name);
+ 		c.people[pos].setAge(this.age);
+ 		this.id := pos;
+ 		this.con := c;
  	}
 
- 	method delete(PersondDB c)
+ 	method delete()
  	modifies this
- 	ensures Transiet()
+ 	requires Persitent()
+ 	ensures Transient()
  	{
+ 		con.delete(this.id);
+ 		this.id := -1;
  	}
 
- 	method close(PersondDB c)
+ 	method close(c:PersonDB)
+ 	requires Persitent()
  	ensures Detatched()
  	{
+ 		this.con := null;
  	}
 
- 	method update(PersondDB c)
+ 	method update(c:PersonDB)
  	modifies this
  	ensures Persitent()
  	{
+ 		this.con := c;
+ 	}
+
+ 	method setName(a:array<char>)
+ 	modifies this
+ 	requires a.Length > 0
+ 	ensures this.name.Length > 0
+ 	{
+ 		this.name := a;
+ 	}
+
+ 	method setAge(n:int)
+ 	modifies this
+ 	requires n >= 0;
+ 	ensures this.age >= 0;
+ 	{
+		this.age := n; 		
+ 	}
+
+ 	method setID(i:int)
+ 	modifies this
+ 	{
+ 		this.id := i;
+ 	}
+
+ 	method setDB(db:PersonDB)
+ 	modifies this
+ 	{
+ 		this.con := db;
  	}
 }
 
@@ -91,10 +169,5 @@ class main
 	{
 		var c:PersonDB := new PersonDB();
 		var p:Person := new Person();
-		c.save(p);
-		p.setName("zé");
-		c.save(p);
-		c.close();
-		c.update(p);
 	}	
 }
